Obtained by transferring a measure from one [[Measurable Space|measurable space]] to another by a [[Measurable Function|measurable function]].

Given: 
- Measurable spaces: ($X_1, \Sigma_1$) and ($X_2, \Sigma_2$)
- Measurable mapping: $f: X_1\rightarrow X_2$
- Measure: $\mu : \Sigma_1 \rightarrow [0, +\infty]$

The pushforward measure of $\mu$, $f_*(\mu):\Sigma_2\rightarrow [0, +\infty]$, is:
$$
f_*(\mu)(B) = \mu(f^{-1}(B))\text{, }B\in \Sigma_2
$$
#DontGetIt 
###### Tags
#MeasureTheory #ProbabilityTheory #FunctionalAnalysis 